progress on range.

src/QuickCodes.fst
@@ -7,32 +7,32 @@ open FStar.List
 
 (** * Comparing [reglist] *)
 
-let rec regs_list_match (#t:reg_t) (regs: list (n:nat{n < n_regtype t})) (r0:regmap) (r1:regmap) : Type0 =
+let rec regs_list_match (#t:reg_t) (regs: list (regtyp t)) (r0:regmap) (r1:regmap) : Type0 =
 match regs with
 | [] -> True
 | r::regs' -> r0 t r == r1 t r /\ regs_list_match regs' r0 r1
 
 unfold
 let reglist_match (t:reg_t)(r0:regmap)(r1:regmap) : Type0 =
-	regs_list_match (reglist t) r0 r1
+  regs_list_match (reglist t) r0 r1
 
 (** * Lemmas about comparing [reglist] *)
 
-val lemma_regs_list_match : #t:reg_t -> regs:list (n:nat{n < n_regtype t}) -> r0:regmap -> r1:regmap -> Lemma
-	(regs_list_match regs r0 r1 ==>
-	 (forall (r:regtyp t). mem r regs ==> r0 t r == r1 t r))
-let rec lemma_regs_list_match #t regs r0 r1 = 
+val lemma_regs_list_match : #t:reg_t -> regs:list (regtyp t) -> r0:regmap -> r1:regmap -> Lemma
+  (regs_list_match regs r0 r1 ==>
+  (forall (r:regtyp t). mem r regs ==> r0 t r == r1 t r))
+let rec lemma_regs_list_match #t regs r0 r1 =
 match regs with
 | [] -> ()
 | r::regs' -> lemma_regs_list_match regs' r0 r1
 
 val lemma_reglist_match : t:reg_t -> r0:regmap -> r1:regmap -> Lemma
-	(reglist_match t r0 r1 ==>
-	 r0 t == r1 t)
-let lemma_reglist_match t r0 r1 = 
-	lemma_regs_list_match (reglist t) r0 r1;
-	lemma_reglist_derive #t (fun r -> r0 t r == r1 t r);
-	assert (reglist_match t r0 r1 ==> equal1 (r0 t) (r1 t))
+  (reglist_match t r0 r1 ==>
+    r0 t == r1 t)
+let lemma_reglist_match t r0 r1 =
+  lemma_regs_list_match (reglist t) r0 r1;
+  lemma_reglist_derive #t (fun r -> r0 t r == r1 t r);
+  assert (reglist_match t r0 r1 ==> equal1 (r0 t) (r1 t))
 
 (** * Comparing [regclasses] *)
 
@@ -41,33 +41,33 @@ match regs with
 | [] -> True
 | t::regs' -> reglist_match t r0 r1 /\ regs_class_match regs' r0 r1
 
-unfold 
+unfold
 let regclasses_match (r0:regmap) (r1:regmap) : Type0 =
-	regs_class_match regclasses r0 r1
+  regs_class_match regclasses r0 r1
 
 (** * Lemmas about comparing [regclasses] *)
 
 val lemma_regs_class_match : regs:(list reg_t) -> r0:regmap -> r1:regmap -> Lemma
-	(regs_class_match regs r0 r1 ==>
-	 (forall t. mem t regs ==> r0 t == r1 t))
+  (regs_class_match regs r0 r1 ==>
+    (forall t. mem t regs ==> r0 t == r1 t))
 let rec lemma_regs_class_match regs r0 r1 =
 match regs with
 | [] -> ()
 | t::regs' -> lemma_reglist_match t r0 r1; lemma_regs_class_match regs' r0 r1
 
 val lemma_regclasses_match : r0:regmap -> r1:regmap -> Lemma
-	(regclasses_match r0 r1 ==>
-	 r0 == r1)
+  (regclasses_match r0 r1 ==>
+    r0 == r1)
 let rec lemma_regclasses_match r0 r1 =
-	lemma_regs_class_match regclasses r0 r1;
-	lemma_regclasses_derive (fun t -> r0 t == r1 t);
-	assert (regclasses_match r0 r1 ==> equal r0 r1)
+  lemma_regs_class_match regclasses r0 r1;
+  lemma_regclasses_derive (fun t -> r0 t == r1 t);
+  assert (regclasses_match r0 r1 ==> equal r0 r1)
 
 (** [va_state_match] *)
 
 let va_state_match (s0:state) (s1:state) : Pure Type0
     (requires True)
     (ensures fun b -> b ==> state_eq s0 s1) =
-	let _ = lemma_regclasses_match s0.regs s1.regs in
+    let _ = lemma_regclasses_match s0.regs s1.regs in
     s0.ok == s1.ok /\
     regclasses_match s0.regs s1.regs
