src/Regs.fsti
@@ -11,28 +11,28 @@ type reg_t = n:nat{n < n_reg_t}
 let regclasses : list reg_t = range n_reg_t
 
 let lemma_regclasses_complete : unit -> Lemma
-	(forall (t:reg_t). mem t regclasses) = fun _ ->
-	lemma_range_complete n_reg_t;
-	assert (forall (t:reg_t). t < n_reg_t)
+  (forall (t:reg_t). mem t regclasses) = fun _ ->
+    lemma_range_complete n_reg_t;
+    assert (forall (t:reg_t). t < n_reg_t)
 
 let lemma_regclasses_derive : p:(reg_t -> Type0) -> Lemma
-	((forall t0. mem t0 regclasses ==> p t0) ==> (forall t. p t)) = fun _ ->
-	lemma_regclasses_complete ()
+  ((forall t0. mem t0 regclasses ==> p t0) ==> (forall t. p t)) = fun _ ->
+    lemma_regclasses_complete ()
 
 val n_regtype : reg_t -> pos
 
-unfold type regtyp (t:reg_t) = n:nat{n < n_regtype t}
+type regtyp (t:reg_t) = n:nat{n < n_regtype t}
 
 (* why [list (regtyp t)] does not work here? *)
-let reglist (t:reg_t) : list (n:nat{n < n_regtype t}) = range (n_regtype t)
+let reglist (t:reg_t) : list (regtyp t) = range (n_regtype t)
 
 let lemma_reglist_complete : t:reg_t -> Lemma
-	(forall (r:regtyp t). mem r (reglist t)) = fun t ->
-	lemma_range_complete (n_regtype t)
+  (forall (r:regtyp t). mem r (reglist t)) = fun t ->
+    lemma_range_complete (n_regtype t)
 
 let lemma_reglist_derive : #t:reg_t -> p:(regtyp t -> Type0) -> Lemma
-	((forall r0. mem r0 (reglist t) ==> p r0) ==> (forall r. p r)) = fun #t p ->
-	lemma_reglist_complete t
+  ((forall r0. mem r0 (reglist t) ==> p r0) ==> (forall r. p r)) = fun #t p ->
+    lemma_reglist_complete t
 
 val regval : reg_t -> Type0
 
@@ -40,10 +40,10 @@ val regval : reg_t -> Type0
 type regmap = t:reg_t -> regtyp t -> regval t
 
 let equal1 (#t:reg_t)(regs1:regtyp t -> regval t)(regs2:regtyp t -> regval t) : Type0 =
-	feq regs1 regs2
+  feq regs1 regs2
 
 let equal (regs1:regmap)(regs2:regmap) : Type0 =
-	forall t. equal1 #t (regs1 t) (regs2 t)
+  forall t. equal1 #t (regs1 t) (regs2 t)
 
 let lemma_equal1_intro : t:reg_t -> regs1:regmap -> regs2:regmap -> Lemma
   (requires forall r. regs1 t r == regs2 t r)
