src/Util.fst
@@ -1,10 +1,39 @@
 module Util
 
-let range (n:nat) : list (m:nat{m < n}) =
-	let rec range' (n':nat{n'<=n}) : list (m:nat{m < n}) =
-		if n' = 0 then [] else (n'-1) :: range' (n'-1) in
-	range' n
+let rec promote (#n:pos) (l:list (m:nat{m < n})) : list (m:nat{m < (n + 1)}) =
+  match l with
+  | [] -> []
+  | hd::tl -> hd::promote tl
 
-let rec range_complete : n:nat -> Lemma
-	(forall m. m < n <==> mem m (range n)) =
-	fun n -> if n = 0 then () else range_complete (n-1)
+let rec promote_preserves_mem : #n:pos -> m:nat{m < n} -> l:list (m:nat{m < n}) -> Lemma
+  (mem m l ==> mem m (promote l)) = fun #n m l ->
+  match l with
+  | [] -> ()
+  | hd::tl -> if m = hd then () else promote_preserves_mem m tl
+
+let rec range (n:pos) : list (m:nat{m < n}) =
+  if n = 1 then [0] else (n-1)::promote (range (n-1))
+
+let range_hd (n:pos) : Tot nat =
+  match range n with
+  | hd::_ -> hd
+
+let rec lemma_range_hd : n:pos -> Lemma
+  (range_hd n = n - 1 /\ mem (range_hd n) (range n)) =
+  fun n -> if n = 1 then () else lemma_range_hd (n-1)
+
+let lemma_mem_cons : n:pos{n > 1} -> m:nat{m < n} -> Lemma
+  (mem m (promote (range (n-1))) ==> mem m (range n)) = fun n m ->
+  assert (mem m (promote (range (n-1))) ==> mem m ((n-1)::promote (range (n - 1))))
+
+let lemma_mem_promote : n:pos -> m:nat{m < n} -> Lemma
+  (mem m (range n) ==> mem m (promote (range n))) = fun n m ->
+  promote_preserves_mem m (range n)
+
+let rec lemma_range_complete n m =
+  match n with
+  | 1 -> ()
+  | _ -> if m = n - 1 then lemma_range_hd n
+        else (lemma_range_complete (n-1) m;
+              lemma_mem_promote (n-1) m;
+              lemma_mem_cons n m)
