src/Util.fsti
@@ -4,5 +4,5 @@ open FStar.List
 
 val range : n:pos -> list (m:nat{m < n})
 
-val lemma_range_complete : n:nat -> Lemma
-	(forall m. m < n <==> mem m (range n))
+val lemma_range_complete : n:pos -> m:nat{m < n} -> Lemma
+  (mem m (range n))
