Makefile
@@ -1,7 +1,32 @@
 FSTAR=fstar.exe
-FSTAR_OPTS=--include src --log_queries --record_hints
+FSTAR_OPTS=--include src --record_hints --use_hints --use_hint_hashes --cache_checked_modules --odir _output
 
-all:
-	$(FSTAR) src/QuickCodes.fst $(FSTAR_OPTS)
+.PHONY: all clean
+all: src/State.fst.checked src/QuickCode.fst.checked src/Regs.fst/checked src/VaCode.fsti.checked src/Util.fst.checked src/QuickCodes.fst.checked src/Util.fsti/checked
+
+clean:
+	rm -rf src/*.checked
+
+src/State.fst.checked: src/Regs.fsti.checked
+	$(FSTAR) src/State.fst $(FSTAR_OPTS)
+
+src/QuickCode.fst.checked: src/VaCode.fsti.checked src/State.fst.checked
+	$(FSTAR) src/QuickCode.fst $(FSTAR_OPTS)
+
+src/Regs.fst.checked: src/Regs.fsti.checked
 	$(FSTAR) src/Regs.fst $(FSTAR_OPTS)
-	$(FSTAR) src/
+
+src/Regs.fsti.checked: src/Util.fsti.checked
+	$(FSTAR) src/Regs.fsti $(FSTAR_OPTS)
+
+src/VaCode.fsti.checked:
+	$(FSTAR) src/VaCode.fsti $(FSTAR_OPTS)
+
+src/Util.fst.checked: src/Util.fsti.checked
+	$(FSTAR) src/Util.fst $(FSTAR_OPTS)
+
+src/QuickCodes.fst.checked: src/QuickCode.fst.checked src/State.fst.checked src/Regs.fsti.checked
+	$(FSTAR) src/QuickCodes.fst $(FSTAR_OPTS)
+
+src/Util.fsti.checked:
+	$(FSTAR) src/Util.fsti $(FSTAR_OPTS)
